chore: cleanup lock

Iris/Iris/HeapLang/Lib/Lock.lean
@@ -10,7 +10,7 @@ open BI
 
 @[expose] public section
 
-class lock (GF : BundledGFunctors) [IrisGS_gen hlc Exp GF] where
+class Lock (GF : BundledGFunctors) [IrisGS_gen hlc Exp GF] where
   newlock : Val
   acquire : Val
   release : Val
@@ -19,11 +19,11 @@ class lock (GF : BundledGFunctors) [IrisGS_gen hlc Exp GF] where
   name : Type
   [lock_name_inhabited : Inhabited name]
 
-  is_lock : lockG GF → name → Val → IProp GF → IProp GF
+  isLock : lockG GF → name → Val → IProp GF → IProp GF
   locked : lockG GF → name → IProp GF
 
-  is_lock_persistent {N} γ lk (R : IProp GF) : Persistent (is_lock N γ lk R)
-  is_lock_iff {N} γ lk (R₁ R₂ : IProp GF) : is_lock N γ lk R₁ ⊢ (▷ □ (R₁ ∗-∗ R₂)) -∗ is_lock N γ lk R₂
+  isLock_persistent {N} γ lk (R : IProp GF) : Persistent (isLock N γ lk R)
+  isLock_iff {N} γ lk (R₁ R₂ : IProp GF) : isLock N γ lk R₁ ⊢ (▷ □ (R₁ ∗-∗ R₂)) -∗ isLock N γ lk R₂
 
   locked_timeless {N} γ : Timeless (locked N γ)
   locked_exclusive {N} γ : locked N γ ∗ locked N γ ⊢@{IProp GF} False
@@ -31,64 +31,62 @@ class lock (GF : BundledGFunctors) [IrisGS_gen hlc Exp GF] where
   -- TODO: redo with texan triples
   newlock_spec_delay_init {N} :
     ⊢ □ ∀ (Φ : Val → IProp GF),
-      (∀ (v : Val) (γ : name), (∀ R E, R ={E}=∗ is_lock N γ v R) -∗ Φ v)
-      -∗ WP hl({newlock} #()) {{ Φ }}
+      (∀ (v : Val) (γ : name), (∀ R E, R ={E}=∗ isLock N γ v R) -∗ Φ v) -∗
+      WP hl({newlock} #()) {{ Φ }}
   acquire_spec {N} γ lk R :
     ⊢ □ ∀ (Φ : Val → IProp GF),
-    is_lock N γ lk R
-    -∗ ((locked N γ ∗ R) -∗ Φ hl_val(#()))
-    -∗ WP hl({acquire} {lk}) {{ Φ }}
+    isLock N γ lk R -∗
+    ((locked N γ ∗ R) -∗ Φ hl_val(#())) -∗
+    WP hl({acquire} {lk}) {{ Φ }}
   release_spec {N} γ lk R :
     ⊢ □ ∀ (Φ : Val → IProp GF),
-    (is_lock N γ lk R) ∗ locked N γ ∗ R
-    -∗ (True -∗ Φ hl_val(#()))
-    -∗ WP hl({release} {lk}) {{ Φ }}
+    (isLock N γ lk R) ∗ locked N γ ∗ R -∗
+    (True -∗ Φ hl_val(#())) -∗
+    WP hl({release} {lk}) {{ Φ }}
 
-instance lock_name_inhabited [IrisGS_gen hlc Exp GF] [lk : lock GF] : Inhabited lk.name :=
+instance instInhabitedLockName [IrisGS_gen hlc Exp GF] [lk : Lock GF] : Inhabited lk.name :=
   lk.lock_name_inhabited
 
 section lemmas
 
-variable [IrisGS_gen hlc Exp GF] [lk : lock GF] (N : lk.lockG GF)
+variable [IrisGS_gen hlc Exp GF] [lk : Lock GF] (N : lk.lockG GF)
 
-instance is_lock_persistent_inst γ v R : Persistent (lk.is_lock N γ v R) :=
-  lk.is_lock_persistent γ v R
+instance instPersistentLockIsLock  γ v R : Persistent (lk.isLock N γ v R) :=
+  lk.isLock_persistent γ v R
 
-instance locked_timeless_inst γ : Timeless (lk.locked N γ) :=
+instance instTimelessLockLocked  γ : Timeless (lk.locked N γ) :=
   lk.locked_timeless γ
 
-theorem is_lock_contractive γ v :
-    OFE.Contractive (lk.is_lock N γ v) := by
+theorem isLock_contractive γ v : OFE.Contractive (lk.isLock N γ v) := by
   rw [contractive_internalEq (PROP := IProp GF)]
   iintro %x₁ %x₂ #HEQ
   iapply prop_ext
   imodintro
   isplit
   · iintro #H
-    iapply lock.is_lock_iff $$ H
+    iapply Lock.isLock_iff $$ H
     iintro !> !>
     irewrite [HEQ]
     · exact ⟨fun _ _ _ h => wandIff_ne.ne h .rfl⟩
     · iapply equiv_wandIff; exact .rfl
   · iintro #H
-    iapply lock.is_lock_iff $$ H
+    iapply Lock.isLock_iff $$ H
     iintro !> !>
     irewrite [HEQ]
     · exact ⟨fun _ _ _ h => wandIff_ne.ne .rfl h⟩
     · iapply equiv_wandIff; exact .rfl
 
-instance is_lock_ne γ v : OFE.NonExpansive (lk.is_lock N γ v) :=
-  letI := is_lock_contractive N γ v
+instance is_lock_ne γ v : OFE.NonExpansive (lk.isLock N γ v) :=
+  letI _ := isLock_contractive N γ v
   OFE.ne_of_contractive _
 
 theorem newlock_spec R :
     ⊢ □ ∀ (Φ : Val → IProp GF),
-    R
-    -∗ (∀ (v : Val) (γ : lk.name), lk.is_lock N γ v R -∗ Φ v)
-    -∗ WP hl({lk.newlock} #()) {{ Φ }} := by
+    R -∗ (∀ (v : Val) (γ : lk.name), lk.isLock N γ v R -∗ Φ v) -∗
+    WP hl({lk.newlock} #()) {{ Φ }} := by
   iintro %Φ !> HR HΦ
   iapply wp_fupd
-  iapply lk.newlock_spec_delay_init $$ %(fun v => iprop(|={⊤}=> Φ v))
+  iapply lk.newlock_spec_delay_init (N := N) $$ %(fun v => iprop(|={⊤}=> Φ v))
   iintro %v %γ Hinit
   imod Hinit $$ %R %⊤ HR
   iapply HΦ $$ Hinit
